more re-factoring and cleanup

examples/HashTable.v
@@ -11,40 +11,31 @@ Module Type HASH_ASSOCIATION.
   Variable key_t : Set.
   Variable value_t : key_t -> Set.
   Variable key_eq_dec : forall (k1 k2:key_t), {k1 = k2} + {k1 <> k2}.
+  Notation "k1 =! k2" := (key_eq_dec k1 k2) (at level 70, right associativity).
   Variable hash : key_t -> nat.
   Variable table_size : nat.
   Variable table_size_gt_zero : table_size > 0.
 End HASH_ASSOCIATION.
 
-(*************************************************************************************)
-(* The hash-table implementation is a functor, parameterized by a HASH_ASSOCIATION,  *)
-(* and a finite map implementation F over the keys and values from HASH_ASSOCIATION. *)
-(* We use F to implement the buckets.                                                *)
-(*************************************************************************************)
-Module HashTable(HA : HASH_ASSOCIATION)
-                (F : FINITE_MAP with Module A := HA) : FINITE_MAP with Module A := HA.
-
-  Require Import Euclid Peano_dec Minus Array.
-  Open Local Scope hprop_scope.
-
-  Module AT <: FINITE_MAP_AT with Module A:=HA.
-    Module A := HA.
-    Module AL := F.AL.
-    Import A AL.
-    Definition fmap_t : Set := array. (* of F.fmap_t's *)
-                                  
-    (* We compose the modulo function from the Peano_dec library with the key hash
+Module HashTableModel(A : HASH_ASSOCIATION).
+  Import A.
+  Module AL := AssocList(A).
+  Export AL.
+  Require Import Euclid Peano_dec Minus.
+  Require Import Array.
+  (* We compose the modulo function from the Peano_dec library with the key hash
      * to get something that's guaranteed to be in range. *)
-    Program Definition hash(k:A.key_t) : nat := modulo HA.table_size HA.table_size_gt_zero (HA.hash k).
+  Program Definition hash(k:A.key_t) : nat := modulo A.table_size A.table_size_gt_zero (A.hash k).
 
-    Ltac simpl_sig := 
+    Ltac simpl_sig := repeat
       match goal with 
         | [|- context [(proj1_sig ?x)]] => destruct x; simpl
         | [H:context [(proj1_sig ?x)] |- _] => destruct x; simpl in H
-      end. 
+        | [H:exists x, _ |- _] => destruct H
+      end; intuition. 
   
-    Lemma hash_below(k:A.key_t) : hash k < HA.table_size.
-    Proof. unfold hash; intros; simpl_sig; destruct e; omega. Qed.
+    Lemma hash_below(k:A.key_t) : hash k < A.table_size.
+    Proof. unfold hash; intros; simpl_sig. Qed.
 
     (* given a list of key value pairs, return only those where the hash of the key equals i *)
     Fixpoint filter_hash (i:nat) (l:alist_t) {struct l} : alist_t := 
@@ -57,6 +48,82 @@ Module HashTable(HA : HASH_ASSOCIATION)
           filter_hash i l'
       end.
 
+    Lemma sub_succ(x y:nat) : S x <= y -> S (y - S x) = y - x.
+    Proof. intros ; omega. Qed.
+
+    Hint Rewrite sub_succ using solve[auto] : AssocListModel.
+    Hint Rewrite <- minus_n_n : AssocListModel.
+
+    (* TODO: split up simpler into model and hash table parts
+     * the model should not need to import Array *)
+    Ltac simpler := subst;
+      repeat (progress ((repeat 
+        match goal with
+          | [|- context [?n - ?n]] => rewrite <- minus_n_n
+          | [|- context [_ + 0]] => rewrite <- plus_n_O
+          | [H:context [_ + 0] |- _] => rewrite <- plus_n_O in H
+          | [|- context [_ - 0]] => rewrite <- minus_n_O
+          | [H:context [_ - 0] |- _] => rewrite <- minus_n_O in H
+(*          | [|- context [?x - ?x]] => rewrite <- minus_n_n
+          | [|- context [S (A.table_size - S ?x)]] => rewrite sub_succ; [idtac | solve[auto]] *)
+          | [H:array_length ?x = _ |- context [array_length ?x]] => rewrite H
+          | [ |- context[if eq_nat_dec ?e1 ?e2 then _ else _] ] => 
+            destruct (eq_nat_dec e1 e2) ; try congruence ; try solve [assert False; intuition]; try subst
+        end); AL.simpler)).
+    Ltac t := repeat (progress (simpler; simpl in *; autorewrite with AssocListModel; auto; intuition)).
+
+    (* some facts about filter_hash *)
+    Lemma filter_hash_lookup k l : lookup k (filter_hash (hash k) l) = lookup k l.
+    Proof. induction l; t. Qed.
+
+    Lemma filter_hash_lookup_none x i l :  lookup x l = None -> lookup x (filter_hash i l) = None.
+    Proof. induction l; t. Qed.
+
+    Lemma filter_hash_perm i l l' : Permutation l l' -> Permutation (filter_hash i l) (filter_hash i l').
+    Proof. induction 1; t; eauto. Qed.
+    Hint Resolve filter_hash_lookup filter_hash_lookup_none.
+
+    Lemma filter_hash_distinct i l : distinct l -> distinct (filter_hash i l).
+    Proof. induction l; t. Qed.
+    Hint Resolve filter_hash_perm filter_hash_distinct.
+
+    Lemma remove_filter_eq (k:A.key_t)(l:alist_t) : 
+      remove k (filter_hash (hash k) l) = filter_hash (hash k) (remove k l).
+    Proof. induction l; t. Qed.
+      
+    Lemma remove_filter_neq (k:A.key_t)(i:nat)(l:alist_t) : 
+      (hash k <> i) -> filter_hash i (remove k l) = filter_hash i l.
+    Proof. induction l ; t. Qed.
+    Hint Rewrite filter_hash_lookup remove_filter_eq : AssocListModel.
+
+    Lemma insert_filter_eq k v (l:alist_t) : 
+      insert v (filter_hash (hash k) l) = (k,,v)::filter_hash (hash k) (remove k l).
+    Proof. unfold insert; t. Qed.
+    Hint Rewrite insert_filter_eq : AssocListModel.
+    Hint Rewrite remove_filter_neq using solve[omega|congruence|t]: AssocListModel.
+
+  End HashTableModel.
+
+(*************************************************************************************)
+(* The hash-table implementation is a functor, parameterized by a HASH_ASSOCIATION,  *)
+(* and a finite map implementation F over the keys and values from HASH_ASSOCIATION. *)
+(* We use F to implement the buckets.                                                *)
+(*************************************************************************************)
+Module HashTable(HA : HASH_ASSOCIATION)
+                (F : FINITE_MAP with Module A := HA) : FINITE_MAP with Module A := HA.
+
+  Open Local Scope hprop_scope.
+  Require Export Array.
+  Require Import Peano_dec.
+
+  Module HL := HashTableModel(HA).
+
+  Module AT <: FINITE_MAP_AT with Module A:=HA.
+    Module A := HA.
+    Module AL := F.AL.
+    Import A AL HL.
+    Definition fmap_t : Set := array. (* of F.fmap_t's *)
+                                  
     (* The ith bucket of a hash-table is well-formed with respect to the association list
      * l, if it points to an F.fmap_t that represents l filtered by i. *)
 
@@ -70,46 +137,17 @@ Module HashTable(HA : HASH_ASSOCIATION)
     Definition rep (f:fmap_t) (l:alist_t) : hprop := 
       [array_length f = HA.table_size] * {@ (wf_bucket f l i) | i <- 0 + HA.table_size}.
 
-    Lemma sub_succ(x:nat) : 
-      S x <= HA.table_size -> S (HA.table_size - S x) = HA.table_size - x.
-    Proof. intros ; omega. Qed.
-
-    Ltac simpler :=
-      repeat (progress ((repeat 
-        match goal with
-          | [H:?e = ?e |- _] => clear H
-          | [|- context [?x - ?x]] => rewrite <- minus_n_n
-          | [|- context [S (HA.table_size - S ?x)]] => rewrite sub_succ; [idtac | solve[auto]]
-          | [H:array_length ?x = _ |- context [array_length ?x]] => rewrite H
-          | [ |- context[if eq_nat_dec ?e1 ?e2 then _ else _] ] => 
-            destruct (eq_nat_dec e1 e2) ; try congruence ; try solve [assert False; intuition]; try subst
-        end); AL.simpler)).
-
-    (* some facts about filter_hash *)
-    Lemma filter_hash_perm i l l' : Permutation l l' -> Permutation (filter_hash i l) (filter_hash i l').
-    Proof. induction 1; simpler; eauto. Qed.
-
-    Lemma filter_hash_lookup k l : lookup k (filter_hash (hash k) l) = lookup k l.
-    Proof. induction l; auto; simpl. destruct a. destruct (eq_nat_dec (hash x) (hash k)); simpl; repeat simpler. Qed.
-
-    Lemma filter_hash_lookup_none x i l :  lookup x l = None -> lookup x (filter_hash i l) = None.
-    Proof. induction l; simpler. Qed.
-    Lemma filter_hash_distinct i l : distinct l -> distinct (filter_hash i l).
-    Proof. Hint Resolve filter_hash_lookup_none. induction l; simpler; intuition. Qed.
-    Hint Resolve filter_hash_perm filter_hash_distinct filter_hash_lookup.
-
   End AT.
 
   Module T:=FINITE_MAP_T(HA)(AT).
 
-  Import AT.
+  Module A := HA.
+  Module AL := F.AL.
+  Import AL AT HL.
   
   Open Local Scope stsepi_scope.
   Open Local Scope hprop_scope.
 
-  Module A := HA.
-  Module AL := F.AL.
-  Import AT AL.
   Ltac s := T.unfm_t; intros.
 
   (* The following is used to initialize an array with empty F.fmap_t's *)
@@ -124,16 +162,6 @@ Module HashTable(HA : HASH_ASSOCIATION)
   Definition free_post (f:array)(n:nat) (_:unit) := {@ p :~~ array_plus f i in ptsto_any p | i <- (HA.table_size - n) + n}.
   Definition free_spec (f:array)(l:[alist_t])(n:nat) := (n <= HA.table_size) -> STsep (free_pre f l n) (free_post f n).
 
-  Lemma add_fact F P Q R : 
-    (P ==> [F] * ??) ->
-    (F -> (P * Q ==> R)) ->
-    (P * Q ==> R).
-  Proof.
-    repeat intro. apply H0; auto. 
-    destruct H1 as [? [? [? [Px ?]]]].
-    destruct (H _ Px) as [? [? [? [[? ?] ?]]]]; trivial.
-  Qed.
-
   (* This should be generalized for all finite maps. *)
   Lemma add_dis (v:F.AT.fmap_t) (l:F.AL.alist_t) P Q : 
     (distinct l -> (F.AT.rep v l * P ==> Q)) ->
@@ -147,10 +175,11 @@ Module HashTable(HA : HASH_ASSOCIATION)
                                          | [H:distinct l |- _] => fail 1
                                          | _ => apply add_dis; intros
                                        end
-                                     end))). 
+                                     end))).
   
   Ltac unf := unfold init_pre, init_post, free_pre, free_post, rep, wf_bucket, ptsto_any.
-  Ltac t := unf; simpl; sep fail ltac:(subst; AT.simpler; unfold_local).
+  Ltac t := unf; simpl; simpler; sep fail ltac:(subst; unfold_local; simpler); 
+    simpler; autorewrite with AssocListModel; sep fail auto.
 
   Definition init_table(f:array)(n:nat) : init_table_spec f n.
   intro.
@@ -158,23 +187,47 @@ Module HashTable(HA : HASH_ASSOCIATION)
     fix init(n:nat) : init_table_spec f n :=
           IfZero n
           Then fun _ => {{Return tt}}
-          Else fun _ => m <- F.new 
-                      <@> init_pre f (S n)
-                  ; upd_array f (HA.table_size - S n) m
-                      <@> (init_pre f n * F.AT.rep m nil_al)
+          Else fun _ => m <- F.new <@> _
+                      ; upd_array f (HA.table_size - S n) m
+                        <@> (init_pre f n * F.AT.rep m nil_al)
                  ;; {{init n _ <@> wf_bucket f nil_al (HA.table_size - S n)}})
-  ; [| | | | t | | | t |]; t. Defined.
+  ; t. Qed.
+(*  ; [| | | | t' | | | t' |]; t'. Qed. *)
 
   (* We allocate an array and then initialize it with empty F.fmap_t's *)
   Definition new : T.new. s.
   refine (  t <- new_array HA.table_size 
-          ; Assert ([array_length t = HA.table_size] * {@hprop_unpack (array_plus t i)
-            (fun p : ptr => Exists A :@ Set, (Exists v :@ A, p --> v)) | i <-
-               (HA.table_size - HA.table_size) + HA.table_size})
-         ;; @init_table t HA.table_size _
-              <@> _ (* [array_length t = HA.table_size] *)
+         ; @init_table t HA.table_size _ <@>  _ 
          ;; {{Return t}})
-  ; t. Defined.
+  ; t. Qed.
+
+
+  (* the following runs through the array and calls F.free on each of the buckets. *)
+  Definition free_table(f:array)(l:[alist_t])(n:nat) : free_spec f l n.
+  intros f l.
+  refine (fix free_tab(n:nat) : free_spec f l n := 
+          match n as n' return free_spec f l n' 
+          with
+          | 0 => fun H => {{Return tt}}
+          | S i => fun H => let j := HA.table_size - S i in
+                              let p := array_plus f j in 
+              fm <- sub_array f j 
+                       (fun fm => l ~~ F.AT.rep fm (filter_hash j l) * 
+                        iter_sep (wf_bucket f l) (HA.table_size - i) i) 
+            ; F.free fm (l ~~~ filter_hash j l)
+                <@> ((p ~~ p --> fm) * free_pre f l i)
+           ;; {{free_tab i _ <@> _}}
+          end)
+  ; clear free_tab; t. 
+Defined.
+
+  (* Run through the array, call F.free on all of the maps, and then call array_free *)
+  Definition free : T.free. s.
+  refine (@free_table x l HA.table_size _ 
+              <@> [array_length x = HA.table_size]
+      ;; free_array x)
+; t. Defined.
+
 
 Lemma iter_imp_f(P1 P2:nat->hprop)(len start:nat) Q R : 
   (forall i, i >= start -> i < len + start -> P1 i ==> P2 i) -> 
@@ -194,41 +247,34 @@ Ltac iter_imp :=
                 end)
         end).
 
-  Hint Resolve hash_below.
-
   Lemma perm : T.perm.
   Proof. Hint Resolve F.perm. s; t; iter_imp; t; add_dis; t. Qed.
+  Hint Resolve hash_below.
 
-  Lemma himp_trans_simpl P Q R : P ==> Q -> Q ==> R -> P ==> R.
-  Proof. firstorder. Qed.
-
-  Lemma himp_trans P Q F1 R : P ==> Q -> Q * F1 ==> R -> P * F1 ==> R.
+  Lemma himp_trans_frame P Q F1 R : P ==> Q -> Q * F1 ==> R -> P * F1 ==> R.
   Proof. firstorder. Qed.
 
   Ltac trans_imp := 
   search_prem ltac:(idtac; 
     match goal with
-      [H:?P ==> ?Q |- ?P * ?F1 ==> ?R] => apply (@himp_trans P Q F1 R H)
+      [H:?P ==> ?Q |- ?P * ?F1 ==> ?R] => apply (@himp_trans_frame P Q F1 R H)
     end).
 
   Lemma iter_sep_inj (len s:nat) P Q  : len > 0 -> {@ Q i * [P] | i <- s + len} ==> {@ Q i | i <- s + len} * [P].
   Proof. induction len; t. assert False; intuition. iter_imp; t. Qed.
 
-  Lemma iter_sep_star_conc (len s:nat) P Q : {@ P i * Q i  | i <- s + len} ==> {@ P i | i <- s + len} * {@ Q i | i <- s + len} .
-  Proof. induction len; t. apply himp_comm_conc. apply IHlen. Qed.
+  Lemma iter_sep_star_conc (len s:nat) P Q : {@ P i * Q i  | i <- s + len} 
+    ==> {@ P i | i <- s + len} * {@ Q i | i <- s + len} .
+  Proof. induction len; t. apply himp_comm_conc. auto. Qed.
 
-  Lemma iter_sep_star_prem (len s:nat) P Q : {@ P i | i <- s + len} * {@ Q i | i <- s + len} ==> {@ P i * Q i  | i <- s + len}.
-  Proof. induction len; t. apply himp_comm_prem. apply IHlen. Qed.
-
-  Lemma star_any_any : ?? * ?? ==> ??.
-  Proof. firstorder. Qed.
-
-  Lemma iter_sep_all_any (len s:nat) :  {@ ?? | i <- s + len} ==> ??.
-  Proof. induction len. t. intros. simpl. pose (IHlen (S s)). trans_imp. apply star_any_any. Qed.
+  Lemma iter_sep_star_prem (len s:nat) P Q : {@ P i | i <- s + len} * {@ Q i | i <- s + len} 
+    ==> {@ P i * Q i  | i <- s + len}.
+  Proof. induction len; t. apply himp_comm_prem. auto. Qed.
 
   Lemma iter_sep_any (len s:nat) P  : {@ P i * ??  | i <- s + len} ==> {@ P i | i <- s + len} * ??.
   Proof. intros. apply himp_empty_prem'.
-  apply (@himp_trans _ _ __ ({@P i | i <- (s) + len} * ??) ((iter_sep_star_conc len s P (fun _ => ??)))). sep fail auto.
+  apply (@himp_trans_frame _ _ __ ({@P i | i <- (s) + len} * ??)
+    ((iter_sep_star_conc len s P (fun _ => ??)))). sep fail auto.
   Qed.
 
   Lemma iter_sep_empty (len s:nat)  : {@ __  | i <- s + len} ==> __.
@@ -246,7 +292,7 @@ Ltac iter_imp :=
     iter_imp; t. trans_imp. t. apply iter_sep_empty.
     destruct a. simpl.
     split_index. apply (hash_below x).
-    AT.simpler.
+    simpler.
     assert (A1:{@[distinct
       (if eq_nat_dec (hash x) i
         then (x,, v) :: filter_hash i l
@@ -264,49 +310,22 @@ Ltac iter_imp :=
     repeat trans_imp; clear A1 A2.
     apply inj_and_conc. rewrite filter_hash_lookup. sep fail auto.
     apply himp_empty_conc'. apply himp_split; apply iter_sep_inj_empty.
-    eapply himp_trans_simpl; [idtac|apply IHl].
+    eapply himp_trans; [idtac|apply IHl].
     apply himp_empty_conc'. eapply sp_index_conc; t.
   Qed.
 
   Lemma distinct_from_parts_any l :{@ [distinct (filter_hash i l)] * ?? | i <- (0) + HA.table_size} ==> [distinct l] * ??.
   Proof. intros.
-    eapply himp_trans_simpl.
+    eapply himp_trans.
     apply iter_sep_any. sep fail auto.
     apply distinct_from_parts.
   Qed.
 
   Lemma distinct : T.distinct.
   Proof. s.
-    eapply himp_trans_simpl; [| apply distinct_from_parts_any].
+    eapply himp_trans; [| apply distinct_from_parts_any].
     t. iter_imp; t. add_dis. t.
   Qed.
-
-  (* the following runs through the array and calls F.free on each of the buckets. *)
-  Definition free_table(f:array)(l:[alist_t])(n:nat) : free_spec f l n.
-  intros f l.
-  refine (fix free_tab(n:nat) : free_spec f l n := 
-          match n as n' return free_spec f l n' 
-          with
-          | 0 => fun H => {{Return tt}}
-          | S i => fun H => let j := HA.table_size - S i in
-                              let p := array_plus f j in 
-              fm <- sub_array f j 
-                       (fun fm => l ~~ F.AT.rep fm (filter_hash j l) * 
-                        iter_sep (wf_bucket f l) (HA.table_size - i) i) 
-            ; F.free fm (l ~~~ filter_hash j l)
-                <@> ((p ~~ p --> fm) * free_pre f l i)
-           ;; {{free_tab i _ <@> (p ~~ ptsto_any p )}}
-          end)
-  ; clear free_tab; t. 
-Defined.
-
-  (* Run through the array, call F.free on all of the maps, and then call array_free *)
-  Definition free : T.free. s.
-  refine (@free_table x l HA.table_size _ 
-              <@> [array_length x = HA.table_size]
-      ;; free_array x)
-  ; t. Defined.
-
  
   Definition its := iter_sep.
   Lemma its_re : its = iter_sep. reflexivity. Qed.
@@ -334,25 +353,9 @@ Defined.
                <@> (l ~~ [array_length x = HA.table_size] * 
                  (let p := array_plus x (hash k) in p ~~ p --> fm) *
                  iter_sep (wf_bucket x l) 0 (hash k) * 
-                 iter_sep (wf_bucket x l) (S (hash k)) (HA.table_size - (hash k) - 1))}});
-   unf; repeat (simpl; init_split; sep fail ltac:(subst; try split_index_; AT.simpler; unfold_local); t).
- Defined.
-
-  Lemma remove_filter_eq (k:A.key_t)(l:alist_t) : 
-    remove k (filter_hash (hash k) l) = filter_hash (hash k) (remove k l).
-  Proof. induction l; AT.simpler. Qed.
-
-  Lemma remove_filter_neq (k:A.key_t)(i:nat)(l:alist_t) : 
-    (hash k <> i) -> filter_hash i l = filter_hash i (remove k l).
-  Proof. induction l ; intros; AT.simpler. rewrite IHl ; auto. Qed.
-    
-  Hint Resolve remove_filter_eq remove_filter_neq.
-
-  Ltac remove_filter_eq := 
-    repeat match goal with 
-    | [|- context [filter_hash ?i (remove ?k _)]] => rewrite <- (@remove_filter_neq k i); [idtac|solve[auto]||omega]
-    | [|- context [F.AT.AL.remove ?k (filter_hash (hash ?k) ?l)]] => rewrite remove_filter_eq
-  end.
+                 iter_sep (wf_bucket x l) (S (hash k)) (HA.table_size - (hash k) - 1))}}); 
+   unf; repeat (simpl; init_split; sep fail ltac:(subst; try split_index_; simpler; unfold_local); t).
+ Qed.
 
   Definition insert : T.insert. s;
   refine (fm <- sub_array x (hash k) (* find the right bucket *)
@@ -369,9 +372,9 @@ Defined.
              (l ~~ (iter_sep (wf_bucket x l) 0 (hash k) * 
                 iter_sep (wf_bucket x l) (S (hash k)) (HA.table_size - (hash k) - 1)))
         }}); 
-  unf; repeat (simpl; init_split; sep fail ltac:(subst; try split_index_; AT.simpler; unfold_local); t); unfold its.
-  repeat (iter_imp;  unfold F.AT.AL.insert; sep fail ltac:(AT.simpler; try remove_filter_eq)).
- Defined.
+  unf; repeat (simpl; init_split; sep fail ltac:(subst; try split_index_; simpler; unfold_local); t); unfold its.
+  repeat (iter_imp; t).
+  Qed.
 
   Definition remove : T.remove. s;
   refine (fm <- sub_array x (hash k) (* find the right bucket *)
@@ -387,8 +390,8 @@ Defined.
              (let p := array_plus x (hash k) in p ~~ p --> fm) * 
              (l ~~ (iter_sep (wf_bucket x l) 0 (hash k) * 
                 iter_sep (wf_bucket x l) (S (hash k)) (HA.table_size - (hash k) - 1)))}}) ; 
-  unf; repeat (simpl; init_split; sep fail ltac:(subst; try split_index_; AT.simpler; unfold_local); t); unfold its.
-  repeat (iter_imp; sep fail ltac:(AT.simpler; try remove_filter_eq)).
- Defined.
+  unf; repeat (simpl; init_split; sep fail ltac:(subst; try split_index_; simpler; unfold_local); t); unfold its.
+  repeat (iter_imp; t).
+  Qed.
 
 End HashTable.
